PAC_Checker2/EPAC_Checker_Synthesis.thy
@@ -119,36 +119,6 @@ sepref_decl_intf ('k, 'b, 'lbl) apac_step is "('k, 'b, 'lbl) pac_step"
 sepref_register merge_cstatus full_normalize_poly new_var is_Add
 
 
-
-lemma is_CL_import[sepref_fr_rules]:
-  assumes \<open>CONSTRAINT is_pure K\<close>  \<open>CONSTRAINT is_pure V\<close> \<open>CONSTRAINT is_pure R\<close>
-  shows
-    \<open>(return o pac_res, RETURN o pac_res) \<in> [\<lambda>x. is_Extension x \<or> is_CL x]\<^sub>a
-       (pac_step_rel_assn K V R)\<^sup>k \<rightarrow> V\<close>
-    \<open>(return o pac_src1, RETURN o pac_src1) \<in> [\<lambda>x. is_Del x]\<^sub>a (pac_step_rel_assn K V R)\<^sup>k \<rightarrow> K\<close>
-    \<open>(return o new_id, RETURN o new_id) \<in> [\<lambda>x. is_Extension x \<or> is_CL x]\<^sub>a (pac_step_rel_assn K V R)\<^sup>k \<rightarrow> K\<close>
-    \<open>(return o is_CL, RETURN o is_CL) \<in>  (pac_step_rel_assn K V R)\<^sup>k \<rightarrow>\<^sub>a bool_assn\<close>
-    \<open>(return o is_Del, RETURN o is_Del) \<in> (pac_step_rel_assn K V R)\<^sup>k \<rightarrow>\<^sub>a bool_assn\<close>
-    \<open>(return o new_var, RETURN o new_var) \<in> [\<lambda>x. is_Extension x]\<^sub>a (pac_step_rel_assn K V R)\<^sup>k \<rightarrow> R\<close>
-    \<open>(return o is_Extension, RETURN o is_Extension) \<in> (pac_step_rel_assn K V R)\<^sup>k \<rightarrow>\<^sub>a bool_assn\<close>
-  using assms
-  by (sepref_to_hoare; sep_auto simp: pac_step_rel_assn_alt_def is_pure_conv ent_true_drop pure_app_eq
-    split: pac_step.splits; fail)+
-
-
-lemma is_CL_import2[sepref_fr_rules]:
-  assumes \<open>CONSTRAINT is_pure K\<close>  \<open>CONSTRAINT is_pure V\<close>
-  shows
-    \<open>(return o pac_srcs, RETURN o pac_srcs) \<in> [\<lambda>x. is_CL x]\<^sub>a (pac_step_rel_assn K V R)\<^sup>k \<rightarrow>  list_assn (V \<times>\<^sub>a K)\<close>
-  using assms
-  by (sepref_to_hoare; sep_auto simp: pac_step_rel_assn_alt_def is_pure_conv ent_true_drop pure_app_eq
-    assms[simplified] list_assn_pure_conv
-    split: pac_step.splits)
-
-lemma is_Mult_lastI:
-  \<open>\<not> is_CL b \<Longrightarrow> \<not>is_Extension b \<Longrightarrow> is_Del b\<close>
-  by (cases b) auto
-
 sepref_register check_linear_combi_l
 sepref_definition check_step_impl
   is \<open>uncurry4 PAC_checker_l_step'\<close>
